FIX axiom to be realized issue

mppa_k1c/PostpassSchedulingOracle.ml
@@ -700,3 +700,11 @@ let schedule bb =
   if debug then (eprintf "###############################\n"; Printf.eprintf "SCHEDULING\n"; print_bb stderr bb);
   (* print_problem (build_problem bb); *)
   if Compopts.optim_postpass () then smart_schedule bb else dumb_schedule bb
+
+(** FIXME - Fix for PostpassScheduling WIP *)
+
+type bblock' = int
+
+let trans_block bb = 1
+
+let bblock_equivb' bb1 bb2 = true
